platform/facade/CompileOut.v
@@ -1,0 +1,41 @@
+Set Implicit Arguments.
+
+Require Import CompileUnit.
+Require Import StringMap WordMap GLabelMap String List.
+Local Open Scope string_scope.
+
+(* the exported Bedrock function and its spec is [export_module_name!fun_name@compileS] *)
+Notation export_module_name := "export".
+Notation extra_stack := 20.
+
+Require Import ADT RepInv.
+Module Make (Import E : ADT) (Import M : RepInv E).
+  Require Import Inv Malloc.
+  Module Import InvMake := Make E.
+  Module Import InvMake2 := Make M.
+  Require Import Semantics.
+
+  Section TopSection.
+
+    (* pre_cond arg1 arg2 *)
+    Variable pre_cond : Value ADTValue -> Value ADTValue -> Prop.
+    (* post_cond arg1 arg2 ret *)
+    Variable post_cond : Value ADTValue -> Value ADTValue -> Value ADTValue -> Prop.
+
+    Definition compileS := SPEC(argvar1, argvar2) reserving (6 + extra_stack)%nat
+      Al v1, Al v2, Al h,                             
+      PRE[V] is_heap h * [| pre_cond v1 v2 /\ let pairs := (V argvar1, v1) :: (V argvar2, v2) :: nil in disjoint_ptrs pairs /\ good_scalars pairs /\ WordMap.Equal h (make_heap pairs) |] * mallocHeap 0
+      POST[R] Ex h', is_heap h' * [| exists r, post_cond v1 v2 r /\ let pairs := (R, r) :: nil in good_scalars pairs /\ WordMap.Equal h' (make_heap pairs) |] * mallocHeap 0.
+
+    Require Import LabelMap.
+
+    Record CompileOut :=
+      {
+        bedrock_module : XCAP.module;
+        bedrock_module_ok : XCAP.moduleOk bedrock_module;
+        bedrock_module_export : LabelMap.find (export_module_name, Labels.Global fun_name) (Exports bedrock_module) = Some (Precondition compileS None)
+      }.
+
+  End TopSection.
+
+End Make.
