platform/facade/CompileUnit.v
@@ -1,7 +1,8 @@
 Set Implicit Arguments.
 
-Require Import DFacade DFModule.
-Require Import StringMap WordMap GLabelMap.
+Require Import DFacade.
+Require Import StringMap WordMap GLabelMap String List.
+Local Open Scope string_scope.
 
 Notation module_name := "dfmodule".
 Notation fun_name := "dffun".
@@ -25,7 +26,10 @@ Section TopSection.
       (* syntax checks, can be discharged by eq_refl for concrete prog *)
       no_assign_to_args : is_disjoint (assigned prog) (StringSetFacts.of_list argvars) = true;
       syntax_ok : is_syntax_ok prog = true;
+      (* will fixed this later *)
+(*
       compile_syntax_ok : FModule.is_syntax_ok (CompileDFacade.compile_op (Build_OperationalSpec argvars retvar prog eq_refl eq_refl no_assign_to_args eq_refl eq_refl syntax_ok)) = true;
+*)
       (* imported axiomatic specs *)
       imports : GLabelMap.t (AxiomaticSpec ADTValue);
       (* correctness conditions *)
@@ -37,44 +41,9 @@ Section TopSection.
       pre_runsto_post : 
         forall st st' value1 value2, 
           StringMap.Equal st (StringMapFacts.make_map (argvar1 :: argvar2 :: nil) (value1 :: value2 :: nil)) -> 
-          pre_cond value1 value2 -> DFacade.RunsTo (GLabelMap.map (@Axiomatic _) imports) prog st st' -> 
+          pre_cond value1 value2 -> 
+          DFacade.RunsTo (GLabelMap.map (@Axiomatic _) imports) prog st st' -> 
           exists ret, StringMapFacts.Submap (StringMapFacts.make_map (retvar :: nil) (ret :: nil)) st' /\ (forall x, x <> retvar -> not_mapsto_adt x st' = true) /\ post_cond value1 value2 ret
     }.
 
 End TopSection.
-
-(* the exported Bedrock function and its spec is [export_module_name!fun_name@compileS] *)
-Notation export_module_name := "export".
-Notation extra_stack := 20.
-
-Require Import ADT RepInv.
-Module Make (Import E : ADT) (Import M : RepInv E).
-  Require Import Inv Malloc.
-  Module Import InvMake := Make E.
-  Module Import InvMake2 := Make M.
-  Require Import Semantics.
-
-  Section TopSection.
-
-    (* pre_cond arg1 arg2 *)
-    Variable pre_cond : Value ADTValue -> Value ADTValue -> Prop.
-    (* post_cond arg1 arg2 ret *)
-    Variable post_cond : Value ADTValue -> Value ADTValue -> Value ADTValue -> Prop.
-
-    Definition compileS := SPEC(argvar1, argvar2) reserving (6 + extra_stack)%nat
-      Al v1, Al v2, Al h,                             
-      PRE[V] is_heap h * [| pre_cond v1 v2 /\ let pairs := (V argvar1, v1) :: (V argvar2, v2) :: nil in disjoint_ptrs pairs /\ good_scalars pairs /\ WordMap.Equal h (make_heap pairs) |] * mallocHeap 0
-      POST[R] Ex h', is_heap h' * [| exists r, post_cond v1 v2 r /\ let pairs := (R, r) :: nil in good_scalars pairs /\ WordMap.Equal h' (make_heap pairs) |] * mallocHeap 0.
-
-    Require Import LabelMap.
-
-    Record CompileOut :=
-      {
-        bedrock_module : XCAP.module;
-        bedrock_module_ok : XCAP.moduleOk bedrock_module;
-        bedrock_module_export : LabelMap.find (export_module_name, Labels.Global fun_name) (Exports bedrock_module) = Some (Precondition compileS None)
-      }.
-
-  End TopSection.
-
-End Make.
